src/Std/Data/Iterators/Lemmas/Combinators.lean
@@ -8,5 +8,6 @@ import Std.Data.Iterators.Lemmas.Combinators.Monadic
 import Std.Data.Iterators.Lemmas.Combinators.Take
 import Std.Data.Iterators.Lemmas.Combinators.TakeWhile
 import Std.Data.Iterators.Lemmas.Combinators.Drop
+import Std.Data.Iterators.Lemmas.Combinators.DropWhile
 import Std.Data.Iterators.Lemmas.Combinators.FilterMap
 import Std.Data.Iterators.Lemmas.Combinators.Zip
