src/Std/Data/Iterators/Lemmas/Combinators/Monadic.lean
@@ -7,5 +7,6 @@ prelude
 import Std.Data.Iterators.Lemmas.Combinators.Monadic.Take
 import Std.Data.Iterators.Lemmas.Combinators.Monadic.TakeWhile
 import Std.Data.Iterators.Lemmas.Combinators.Monadic.Drop
+import Std.Data.Iterators.Lemmas.Combinators.Monadic.DropWhile
 import Std.Data.Iterators.Lemmas.Combinators.Monadic.FilterMap
 import Std.Data.Iterators.Lemmas.Combinators.Monadic.Zip
