src/Std/Data/Iterators/Lemmas/Combinators/Monadic/DropWhile.lean
@@ -1,0 +1,172 @@
+/-
+Copyright (c) 2025 Lean FRO, LLC. All rights reserved.
+Released under Apache 2.0 license as described in the file LICENSE.
+Authors: Paul Reichert
+-/
+prelude
+import Std.Data.Iterators.Combinators.Monadic.DropWhile
+import Std.Data.Iterators.Lemmas.Consumers.Monadic
+
+namespace Std.Iterators
+
+theorem IterM.Intermediate.dropWhileM_eq_dropWhileWithProof {α m β} [Monad m]
+    [Iterator α m β] {it : IterM (α := α) m β} {P dropping} :
+    Intermediate.dropWhileM P dropping it =
+      Intermediate.dropWhileWithProof (monadLift ∘ P) dropping it :=
+  rfl
+
+theorem IterM.Intermediate.dropWhile_eq_dropWhileM {α m β} [Monad m]
+    [Iterator α m β] {it : IterM (α := α) m β} {P} :
+    Intermediate.dropWhile P dropping it =
+      Intermediate.dropWhileM (pure ∘ ULift.up ∘ P) dropping it :=
+  rfl
+
+theorem IterM.dropWhileWithProof_eq_intermediateDropWhileWithProof {α m β}
+    [Iterator α m β] {it : IterM (α := α) m β} {P} :
+    it.dropWhileWithProof P = Intermediate.dropWhileWithProof P true it :=
+  rfl
+
+theorem IterM.dropWhileM_eq_intermediateDropWhileM {α m β} [Monad m]
+    [Iterator α m β] {it : IterM (α := α) m β} {P} :
+    it.dropWhileM P = Intermediate.dropWhileM P true it :=
+  rfl
+
+theorem IterM.dropWhile_eq_intermediateDropWhile {α m β} [Monad m]
+    [Iterator α m β] {it : IterM (α := α) m β} {P} :
+    it.dropWhile P = Intermediate.dropWhile P true it :=
+  rfl
+
+theorem IterM.step_intermediateDropWhileWithProof {α m β} [Monad m] [Iterator α m β]
+    {it : IterM (α := α) m β} {P} {dropping} :
+    (IterM.Intermediate.dropWhileWithProof P dropping it).step = (do
+    match ← it.step with
+    | .yield it' out h =>
+      if h' : dropping = true then
+        match ← (P out).operation with
+        | ⟨.up true, h''⟩ =>
+          return .skip (IterM.Intermediate.dropWhileWithProof P true it') (.dropped h h' h'')
+        | ⟨.up false, h''⟩ =>
+          return .yield (IterM.Intermediate.dropWhileWithProof P false it') out (.start h h' h'')
+      else
+        return .yield (IterM.Intermediate.dropWhileWithProof P false it') out
+            (.yield h (Bool.not_eq_true _ ▸ h'))
+    | .skip it' h =>
+      return .skip (IterM.Intermediate.dropWhileWithProof P dropping it') (.skip h)
+    | .done h =>
+      return .done (.done h)) := by
+  simp only [dropWhileWithProof, step, Iterator.step, internalState_toIterM]
+  apply bind_congr
+  intro step
+  cases step using PlausibleIterStep.casesOn <;> rfl
+
+theorem IterM.step_dropWhileWithProof {α m β} [Monad m] [Iterator α m β]
+    {it : IterM (α := α) m β} {P} :
+    (it.dropWhileWithProof P).step = (do
+    match ← it.step with
+    | .yield it' out h =>
+        match ← (P out).operation with
+        | ⟨.up true, h''⟩ =>
+          return .skip (IterM.Intermediate.dropWhileWithProof P true it') (.dropped h rfl h'')
+        | ⟨.up false, h''⟩ =>
+          return .yield (IterM.Intermediate.dropWhileWithProof P false it') out (.start h rfl h'')
+    | .skip it' h =>
+      return .skip (IterM.Intermediate.dropWhileWithProof P true it') (.skip h)
+    | .done h =>
+      return .done (.done h)) := by
+  simp [dropWhileWithProof_eq_intermediateDropWhileWithProof, step_intermediateDropWhileWithProof]
+
+theorem IterM.step_intermediateDropWhileM {α m β} [Monad m] [LawfulMonad m] [Iterator α m β]
+    {it : IterM (α := α) m β} {P} {dropping} :
+    (IterM.Intermediate.dropWhileM P dropping it).step = (do
+    match ← it.step with
+    | .yield it' out h =>
+      if h' : dropping = true then
+        match ← P out with
+        | .up true =>
+          return .skip (IterM.Intermediate.dropWhileM P true it') (.dropped h h' True.intro)
+        | .up false =>
+          return .yield (IterM.Intermediate.dropWhileM P false it') out (.start h h' True.intro)
+      else
+        return .yield (IterM.Intermediate.dropWhileM P false it') out
+            (.yield h (Bool.not_eq_true _ ▸ h'))
+    | .skip it' h =>
+      return .skip (IterM.Intermediate.dropWhileM P dropping it') (.skip h)
+    | .done h =>
+      return .done (.done h)) := by
+  simp only [Intermediate.dropWhileM_eq_dropWhileWithProof, step_intermediateDropWhileWithProof]
+  apply bind_congr
+  intro step
+  cases step using PlausibleIterStep.casesOn
+  · simp only [Function.comp_apply, PostconditionT.operation_monadLift, PlausibleIterStep.skip,
+    PlausibleIterStep.yield, bind_map_left]
+    split
+    · apply bind_congr
+      rintro ⟨x⟩
+      cases x <;> rfl
+    · rfl
+  · rfl
+  · rfl
+
+theorem IterM.step_dropWhileM {α m β} [Monad m] [LawfulMonad m] [Iterator α m β]
+    {it : IterM (α := α) m β} {P} :
+    (it.dropWhileM P).step = (do
+    match ← it.step with
+    | .yield it' out h =>
+      match ← P out with
+      | .up true =>
+        return .skip (IterM.Intermediate.dropWhileM P true it') (.dropped h rfl True.intro)
+      | .up false =>
+        return .yield (IterM.Intermediate.dropWhileM P false it') out (.start h rfl True.intro)
+    | .skip it' h =>
+      return .skip (IterM.Intermediate.dropWhileM P true it') (.skip h)
+    | .done h =>
+      return .done (.done h)) := by
+  simp [dropWhileM_eq_intermediateDropWhileM, step_intermediateDropWhileM]
+
+theorem IterM.step_intermediateDropWhile {α m β} [Monad m] [LawfulMonad m] [Iterator α m β]
+    {it : IterM (α := α) m β} {P} {dropping} :
+    (IterM.Intermediate.dropWhile P dropping it).step = (do
+    match ← it.step with
+    | .yield it' out h =>
+      if h' : dropping = true then
+        match P out with
+        | true =>
+          return .skip (IterM.Intermediate.dropWhile P true it') (.dropped h h' True.intro)
+        | false =>
+          return .yield (IterM.Intermediate.dropWhile P false it') out (.start h h' True.intro)
+      else
+        return .yield (IterM.Intermediate.dropWhile P false it') out
+            (.yield h (Bool.not_eq_true _ ▸ h'))
+    | .skip it' h =>
+      return .skip (IterM.Intermediate.dropWhile P dropping it') (.skip h)
+    | .done h =>
+      return .done (.done h)) := by
+  simp only [Intermediate.dropWhile_eq_dropWhileM, step_intermediateDropWhileM]
+  apply bind_congr
+  intro step
+  cases step using PlausibleIterStep.casesOn
+  · simp only [Function.comp_apply, PostconditionT.operation_monadLift, PlausibleIterStep.skip,
+    PlausibleIterStep.yield, bind_map_left]
+    split
+    · cases P _ <;> simp
+    · rfl
+  · rfl
+  · rfl
+
+theorem IterM.step_dropWhile {α m β} [Monad m] [LawfulMonad m] [Iterator α m β]
+    {it : IterM (α := α) m β} {P} :
+    (it.dropWhile P).step = (do
+    match ← it.step with
+    | .yield it' out h =>
+        match P out with
+        | true =>
+          return .skip (IterM.Intermediate.dropWhile P true it') (.dropped h rfl True.intro)
+        | false =>
+          return .yield (IterM.Intermediate.dropWhile P false it') out (.start h rfl True.intro)
+    | .skip it' h =>
+      return .skip (IterM.Intermediate.dropWhile P true it') (.skip h)
+    | .done h =>
+      return .done (.done h)) := by
+  simp [dropWhile_eq_intermediateDropWhile, step_intermediateDropWhile]
+
+end Std.Iterators
